demo/fib/Fib67proof.v
@@ -1,0 +1,50 @@
+Require Import CoqlibC Maps Postorder.
+Require Import AST Linking.
+Require Import ValuesC MemoryC GlobalenvsC Events Smallstep.
+Require Import Op ClightC.
+Require Import CtypesC CtypingC.
+Require Import sflib.
+Require Import IntegersC.
+
+Require Import Simulation.
+Require Import Skeleton Mod ModSem SimMod SimModSemLift SimSymb SimMemLift MatchSimModSemExcl.
+Require SoundTop.
+Require SimMemId.
+Require Import Any.
+Require Import SIR.
+Require Import FibHeader.
+Require Import Fib7.
+Require Import Fib6.
+Require Import ModSemProps.
+Require Import Program.
+Require Import SIRProps.
+
+Set Implicit Arguments.
+
+
+
+Theorem correct: rusc defaultR [Fib7.module: Mod.t] [Fib6.module: Mod.t].
+Proof.
+  etrans.
+  {
+    instantiate (1:= [_]).
+    instantiate (1:= SMod.mk Fib0.module _ "fib" FibHeader.initial_owned_heap _).
+    instantiate (2:= (add Fib0._fib (fun _ _ _ => _) empty)).
+    eapply SIREutt.correct; ss; et.
+    cbn. ii; clarify; rr; ss; des_ifs; ss; ii; clarify.
+    r. unfold Fib7.f_fib. do 2 setoid_rewrite <- tau_eutt at 2. refl.
+  }
+  eapply SIRLocal.correct; ss; et.
+  cbn. ii; clarify; rr; ss; des_ifs; ss; ii; clarify.
+  unfold Fib7.f_fib, f_fib.
+  unfold unwrapU. des_ifs; irw; cycle 1.
+  { unfold triggerUB. irw. pfold. econs; et. }
+  unfold assume, precond. des_ifs; cycle 1.
+  { contradict n0. eauto. }
+  des; clarify.
+  irw. pfold. econs; et; cycle 1.
+  { eexists. eexists (_, (_, _)). ss. des_ifs. }
+  ii. destruct x_tgt; ss. destruct x as [ohr [mr vr]]. ss. des_ifs. des; clarify. left. pfold. econs; et.
+Unshelve.
+  all: (by ii; ss; unfold internals in *; des_ifs; eapply_all_once prog_defmap_image; ss; des; clarify).
+Qed.
