demo/fib/Fib78proof.v
@@ -1,0 +1,63 @@
+Require Import CoqlibC Maps Postorder.
+Require Import AST Linking.
+Require Import ValuesC MemoryC GlobalenvsC Events Smallstep.
+Require Import Op ClightC.
+Require Import CtypesC CtypingC.
+Require Import sflib.
+Require Import IntegersC.
+
+Require Import Simulation.
+Require Import Skeleton Mod ModSem SimMod SimModSemLift SimSymb SimMemLift MatchSimModSemExcl.
+Require SoundTop.
+Require SimMemId.
+Require Import Any.
+Require Import SIR.
+Require Import FibHeader.
+Require Import Fib8.
+Require Import Fib7.
+Require Import ModSemProps.
+Require Import Program.
+Require Import SIRProps.
+Require Import MatchSimModSemExcl.
+
+Set Implicit Arguments.
+
+
+Let mp: ModPair.t := (SimSymbId.mk_mp Fib8.module Fib7.module).
+Theorem correct: rusc defaultR [Fib8.module: Mod.t] [Fib7.module: Mod.t].
+Proof.
+  eapply AdequacyLocal.relate_single_rusc; try exists mp; esplits; eauto.
+  econs; ss; et. ii. exists (SimMemOh_default_aux _ (Some "fib")).
+  econs; ss; et.
+  { apply SoundTop.sound_state_local_preservation; et. }
+  { ii. eapply Preservation.local_preservation_noguarantee_weak.
+    apply SoundTop.sound_state_local_preservation; et.
+  }
+  { ii. esplits; et. }
+  { ii. ss. esplits; et.
+    - ii. inv INITTGT. ss. des_ifs. inv SIMSKENV; ss. r in SIMSKE. r in SIMSKELINK. clarify.
+      rr in SIMARGS; des. ss. clarify. inv SIMARGS0; ss. clarify. clear_tac.
+      assert(fid = Fib0._fib).
+      { admit "ez - UNSYMB". }
+      clarify. inv SAFESRC. ss. clarify.
+      esplits; et.
+      { econs; ss; et. }
+      pfold. econs 4; try refl; ss; et.
+      { econs; ss. unfold interp_program, mrec. irw. des_ifs. unfold f_fib. irw.
+        unfold unwrapU. des_ifs. }
+      econs; ss; et. econs; ss; et.
+    - i; des. inv SAFESRC. ss. destruct args_src; ss. clarify.
+      rr in SIMARGS; des. ss. clarify. inv SIMARGS0; ss. clarify. ss. des_ifs. clear_tac.
+      inv SIMSKENV. ss. r in SIMSKE. r in SIMSKELINK. clarify.
+      esplits; ss; et.
+      econs; ss; et.
+      + assert(sg_init_src = signature_of_function Fib0.f_fib).
+        { admit "ez - sig". }
+        clarify. unfold signature_of_function. ss. econs; ss; et.
+        unfold typify_list. cbn. unfold typify. des_ifs; ss.
+      + econs; ss; et.
+  }
+Unshelve.
+- apply unit.
+- apply (Ord.lift_idx unit_ord_wf tt).
+Qed.
