demo/fib/Fib8.v
@@ -1,0 +1,66 @@
+Require Import CoqlibC Maps.
+Require Import ASTC Integers ValuesC EventsC MemoryC Globalenvs.
+Require Import Op Registers.
+Require Import sflib.
+Require Import SmallstepC.
+Require Export Simulation.
+Require Import Skeleton Mod ModSem.
+Require ClightC.
+Require Import FibHeader.
+Require Import Fib0.
+
+Set Implicit Arguments.
+
+Local Obligation Tactic := ii; ss; des; inv_all_once; repeat des_u; ss; clarify.
+
+
+
+Section MODSEM.
+
+  Variable skenv_link: SkEnv.t.
+  Variable p: unit.
+  Let skenv: SkEnv.t := (SkEnv.project skenv_link) Fib0.module.
+
+  Inductive state: Type :=
+  | State
+      (n: nat)
+      (m: mem)
+  .
+
+  Inductive initial_frame (args: Args.t): state -> Prop :=
+  | initial_frame1_intro
+      i m blk n
+      (SYMB: Genv.find_symbol skenv _fib = Some blk)
+      (FPTR: (Args.fptr args) = Vptr blk Ptrofs.zero)
+      (VS: (Args.vs args) = [Vint i])
+      (NAT: to_nat_opt i = Some n)
+      (M: (Args.m args) = m)
+    :
+      initial_frame args (State n m)
+  .
+
+  Inductive final_frame: state -> Retv.t -> Prop :=
+  | final_frame_return
+      n m
+    :
+      final_frame (State n m) (Retv.mk (Vint (of_nat (fib_nat n))) m)
+  .
+
+  Program Definition modsem: ModSem.t :=
+    {|
+      ModSem.step := bot5;
+      ModSem.at_external := bot3;
+      ModSem.initial_frame := coerce initial_frame;
+      ModSem.final_frame := coerce final_frame;
+      ModSem.after_external := bot4;
+      ModSem.globalenv := skenv;
+      ModSem.skenv := skenv;
+      ModSem.skenv_link := skenv_link;
+      ModSem.midx := Some "fib";
+    |}
+  .
+
+End MODSEM.
+
+Program Definition module: Mod.t :=
+  {| Mod.data := tt; Mod.get_sk := fun _ => Fib0.module; Mod.get_modsem := modsem; Mod.midx := Some "fib" |}.
