demo/fib/FibHeader.v
@@ -74,3 +74,6 @@ Global Opaque Z.of_nat.
 
 
 Definition _fib_ru := 57%positive.
+
+Global Obligation Tactic :=
+  try (by ii; ss; unfold internals in *; des_ifs; eapply_all_once prog_defmap_image; ss; des; clarify).
