specIR/SIREutt.v
@@ -306,8 +306,12 @@ Hint Unfold match_itr match_fn match_prog.
 
 Section SIM.
 
-  Variable p_src: program owned_heap.
-  Variable p_tgt: program owned_heap.
+  Variable md_src: SMod.t owned_heap.
+  Variable md_tgt: SMod.t owned_heap.
+  Let p_src := md_src.(SMod.prog).
+  Let p_tgt := md_tgt.(SMod.prog).
+  Let mi_src := md_src.(SMod.midx).
+  Let mi_tgt := md_tgt.(SMod.midx).
   Hypothesis (SIMP: match_prog p_src p_tgt).
 
   Lemma match_itr_glue
@@ -319,7 +323,7 @@ Section SIM.
   Proof.
     eapply Proper_interp_mrec; eauto.
     ii.
-    destruct a. cbn. rr in SIMP. repeat spc SIMP. hexploit1 SIMP; ss. des_ifs.
+    destruct a. cbn. r in SIMP. repeat spc SIMP. hexploit1 SIMP; ss. des_ifs.
     - eapply SIMP; ss.
     - refl.
   Qed.
@@ -421,26 +425,27 @@ Section SIM.
     {
       ii.
       eapply match_prog_sim_st; ss.
-      hexploit (@SIMP fname); et. intro T. rr in T. des_ifs; cycle 1.
+      hexploit (@SIMP fname); et. intro T. r in T. des_ifs; cycle 1.
       { r. refl. }
       repeat (spc T). exploit T; ss; et.
     }
   Qed.
 
-  Variable ioh: SkEnv.t -> owned_heap.
-  Variable sk: Sk.t.
-  Let md_src: Mod.t := (SIR.module sk p_src mi ioh).
-  Let md_tgt: Mod.t := (SIR.module sk p_tgt mi ioh).
+  Hypothesis (SIMMI: mi_src = mi_tgt).
+  Hypothesis (SIMO: forall skenv, (md_src.(SMod.initial_owned_heap) skenv)
+                                  = (md_tgt.(SMod.initial_owned_heap) skenv)).
+  Hypothesis (SIMSK: md_src.(SMod.sk) = md_tgt.(SMod.sk)).
   Let mp: ModPair.t := (SimSymbId.mk_mp md_src md_tgt).
 
   Theorem sim_mod: ModPair.sim mp.
   Proof.
-    eapply SimSIR.sim_mod with (SO:=eq); eauto.
+    eapply SimSIR.sim_mod; eauto.
+    econs; eauto.
     { eapply ord_lex_wf; eapply lt_wf. }
     ii. clarify. esplits. eapply adequacy_local_local; et.
   Qed.
 
-  Theorem correct: rusc defaultR [md_src] [md_tgt].
+  Theorem correct: rusc defaultR [md_src: Mod.t] [md_tgt: Mod.t].
   Proof. eapply AdequacyLocal.relate_single_rusc; try exists mp; esplits; eauto using sim_mod. Qed.
 
 End SIM.
